Port prev commit to feature/targetproof version, other fixes

stanfrontend/CStan.v
@@ -251,12 +251,12 @@ Inductive deref_loc (ty: type) (m: mem) (b: block) (ofs: ptrofs) :
       load_bitfield ty sz sg pos width m (Vptr b ofs) v ->
       deref_loc ty m b ofs (Bits sz sg pos width) v.
 
-Inductive assign_loc (ce: composite_env) (ty: Ctypes.type) (m: mem) (b: block) (ofs: ptrofs):
-                                            val -> mem -> Prop :=
+Inductive assign_loc (ce: composite_env) (ty: type) (m: mem) (b: block) (ofs: ptrofs):
+                                            bitfield -> val -> mem -> Prop :=
   | assign_loc_value: forall v chunk m',
       access_mode ty = By_value chunk ->
       Mem.storev chunk m (Vptr b ofs) v = Some m' ->
-      assign_loc ce ty m b ofs v m'
+      assign_loc ce ty m b ofs Full v m'
   | assign_loc_copy: forall b' ofs' bytes m',
       access_mode ty = By_copy ->
       (sizeof ce ty > 0 -> (alignof_blockcopy ce ty | Ptrofs.unsigned ofs')) ->
@@ -266,5 +266,7 @@ Inductive assign_loc (ce: composite_env) (ty: Ctypes.type) (m: mem) (b: block) (
               \/ Ptrofs.unsigned ofs + sizeof ce ty <= Ptrofs.unsigned ofs' ->
       Mem.loadbytes m b' (Ptrofs.unsigned ofs') (sizeof ce ty) = Some bytes ->
       Mem.storebytes m b (Ptrofs.unsigned ofs) bytes = Some m' ->
-      assign_loc ce ty m b ofs (Vptr b' ofs') m'.
-
+      assign_loc ce ty m b ofs Full (Vptr b' ofs') m'
+  | assign_loc_bitfield: forall sz sg pos width v m' v',
+      store_bitfield ty sz sg pos width m (Vptr b ofs) v m' v' ->
+      assign_loc ce ty m b ofs (Bits sz sg pos width) v m'.
