stanfrontend/Targetproof.v
@@ -25,6 +25,9 @@ Hypothesis TRANSF: Target.transf_program prog = OK tprog.
 Let ge := globalenv prog.
 Let tge := globalenv tprog.
 
+Definition match_temps tgt (le1 le2: temp_env) : Prop :=
+  (forall i v, i <> tgt -> le1!i = Some v -> le2!i = Some v).
+
 Definition get_blockstate (bs : CStanSemanticsTarget.block_state) : blocktype :=
 match bs with
 | CStanSemanticsTarget.Other => BTOther
@@ -52,31 +55,33 @@ Inductive match_cont : blocktype -> cont -> cont -> Prop :=
   | match_Kswitch: forall k tk bt ,
       match_cont bt k tk ->
       match_cont bt (Kswitch k) (Kswitch tk)
-  | match_Kcall: forall optid fn e le k tfn tk bt,
+  | match_Kcall: forall optid fn e le k tfn tle tk bt,
       transf_function (prog_target prog) fn = OK tfn ->
+      match_temps (prog_target prog) le tle ->
       bt <> BTModel ->
       match_cont fn.(fn_blocktype) k tk ->
       match_cont bt (Kcall optid fn e le k)
                         (Kcall optid tfn e le tk)
-  | match_Kcall_model: forall optid fn e le k tfn tk bt,
+  | match_Kcall_model: forall optid fn e le k tfn tle tk bt,
       transf_function (prog_target prog) fn = OK tfn ->
+      match_temps (prog_target prog) le tle ->
       bt = BTModel ->
       match_cont fn.(fn_blocktype) k tk ->
       match_cont bt (Kcall optid fn e le k)
-                        (Kseq (Sreturn (Some (Evar (prog_target prog) tdouble))) (Kcall optid tfn e le tk))
-. (* NOTE: target register is updated local environment -- assuming e and le are identical is probably wrong.*)
-
+                        (Kseq (Sreturn (Some (Etempvar (prog_target prog) tdouble))) (Kcall optid tfn e le tk))
+.
 
 Inductive match_states: CStanSemanticsTarget.state -> CStanSemanticsBackend.state -> Prop :=
   | match_regular_states:
-      forall f s k e le m tf ts tk bs
+      forall f s k e le m tf ts tk tle bs
       (TRF: transf_function (prog_target prog) f = OK tf)
       (TRS: transf_statement (prog_target prog) s = OK ts)
       (BS_OTHER: bs = CStanSemanticsTarget.Other)
       (BS_SYNC: f.(fn_blocktype) = BTOther)
+      (MTMP: match_temps (prog_target prog) le tle)
       (MCONT: match_cont (get_blockstate bs) k tk),
       match_states (CStanSemanticsTarget.State f s k e le m bs)
-                   (CStanSemanticsBackend.State tf ts tk e le m)
+                   (CStanSemanticsBackend.State tf ts tk e tle m)
   | match_call_state:
       forall fd vargs k m tfd tk bs
       (TRFD: transf_fundef (prog_target prog) fd = OK tfd)
@@ -92,15 +97,18 @@ Inductive match_states: CStanSemanticsTarget.state -> CStanSemanticsBackend.stat
                    (CStanSemanticsBackend.Returnstate v tk m)
 
   | match_regular_states_model:
-      forall f s k e le m tf ts tk bs ta
+      forall f s k e le m tf ts tk tle bs ta
       (TRF: transf_function (prog_target prog) f = OK tf)
       (TRS: transf_statement (prog_target prog) s = OK ts)
+      (* (TREPI: exists a, transf_etarget_expr (prog_target prog) a = OK (Etempvar (prog_target prog) tdouble)) *)
+      (* (TCAST:  Cop.sem_cast (Vfloat ta) tdouble (fn_return tf) m = Some (Vfloat ta)) *)
       (BS_MODEL: bs = CStanSemanticsTarget.Model ta)
       (BS_SYNC: f.(fn_blocktype) = BTModel)
-      (TAR_MATCH: le!(prog_target prog)  = Some (Vfloat ta))
+      (TAR_MATCH: le!(prog_target prog) = Some (Vfloat ta)) (* FIXME: needs to access e, but also lookup block in memory*)
+      (MTMP: match_temps (prog_target prog) le tle)
       (MCONT: match_cont (get_blockstate bs) k tk),
       match_states (CStanSemanticsTarget.State f s k e le m bs)
-                   (CStanSemanticsBackend.State tf ts tk e le m)
+                   (CStanSemanticsBackend.State tf ts tk e tle m)
   (* | match_call_state_model: *)
   (*     forall fd vargs k m tfd tk bs fn *)
   (*     (GET_FN: fd = Internal fn) *)
@@ -125,6 +133,26 @@ Definition match_prog (p: CStan.program) (tp: CStan.program) :=
     match_program (fun ctx f tf => Target.transf_fundef p.(prog_target) f = OK tf) eq p tp
  /\ prog_types tp = prog_types p.
 
+Lemma match_temps_assign_tgt:
+  forall tgt le te id v,
+  tgt = id ->
+  match_temps tgt le te ->
+  match_temps tgt le (PTree.set id v te).
+Proof.
+  intros tgt le te id v Heq Hmatch.
+  red; intros. rewrite PTree.gsspec in *. subst. destruct (peq i id); auto.
+  congruence.
+Qed.
+
+Lemma match_temps_assign:
+  forall tgt le te id v,
+  match_temps tgt le te ->
+  match_temps tgt (PTree.set id v le) (PTree.set id v te).
+Proof.
+  intros tgt le te id v Hmatch.
+  red; intros. rewrite PTree.gsspec in *. destruct (peq i id); auto.
+Qed.
+
 Variable TRANSL: match_prog prog tprog.
 
 Lemma comp_env_preserved:
@@ -137,14 +165,14 @@ Proof.
   congruence.
 Qed.
 
-(* Inductive tr_function: CStan.function -> CStan.function -> Prop := *)
-(*   | tr_function_intro: forall f tf, *)
-(*       (* tr_stmt f.(CStan.fn_body) tf.(fn_body) -> *) *)
-(*       fn_return tf = CStan.fn_return f -> *)
-(*       fn_callconv tf = CStan.fn_callconv f -> *)
-(*       fn_params tf = CStan.fn_params f -> *)
-(*       fn_vars tf = CStan.fn_vars f -> *)
-(*       tr_function f tf. *)
+Inductive tr_function: CStan.function -> CStan.function -> Prop :=
+  | tr_function_intro: forall f tf,
+      (* tr_stmt f.(CStan.fn_body) tf.(fn_body) -> *)
+      fn_return tf = CStan.fn_return f ->
+      fn_callconv tf = CStan.fn_callconv f ->
+      fn_params tf = CStan.fn_params f ->
+      fn_vars tf = CStan.fn_vars f ->
+      tr_function f tf.
 
 (* Inductive tr_fundef: CStan.fundef -> Clight.fundef -> Prop := *)
 (*   | tr_internal: forall f tf, *)
@@ -200,17 +228,25 @@ Proof.
 
     (* cases with inductive hypothesis: Ederef, Eunop, Ebinop *)
     try (monadInv H1;  (* invert our inductive transf_expression *)
-         constructor). (* the rest of the proof follows precisely by constructor *)
+         constructor).
+
+    try (destruct (Pos.eqb _ _); monadInv H1; constructor).
 Qed.
 
 Lemma eval_expr_correct:
-  forall e le m a v bs ta
-  (TRE: Target.transf_etarget_expr (prog_target prog)  a = OK ta),
-  CStanSemanticsTarget.eval_expr ge e le m bs a v -> eval_expr tge e le m ta v.
+  forall e le tle m a v bs ta
+   (TAR: match bs with
+         | CStanSemanticsTarget.Other => True
+         | CStanSemanticsTarget.Model tv => tle!(prog_target prog) = Some (Vfloat tv)
+         end)
+   (MTMP: match_temps (prog_target prog) le tle)
+   (TRE: Target.transf_etarget_expr (prog_target prog) a = OK ta),
+  CStanSemanticsTarget.eval_expr ge e le m bs a v ->
+  eval_expr tge e tle m ta v.
 Proof.
-  intros e le m a.
+  intros e le tle m a.
   induction a; intros;
-  simpl in TRE; monadInv TRE; simpl.
+  simpl in TRE; try monadInv TRE; simpl.
     (* Econsts *)
   - inv H; try constructor; inv H0.
   - inv H; try constructor; inv H0.
@@ -226,38 +262,61 @@ Proof.
     rewrite symbols_preserved; eauto.
 
   - (* Etempvar *)
-    inv H. constructor; eauto. inv H0.
+    destruct (Pos.eqb_spec i (prog_target prog)); try monadInv TRE; [].
+    simpl. inv H.
+    * constructor; eauto.
+    * inversion H0.
   - (* Ederef *)
-    inv H. inv H0.
-  - (*Ecast*)
-    admit. (* inv H3. *)
-    (* apply (IHa v bs ta i). *)
-  (*   monadInv TRE. *)
-  (*   eapply IHa. *)
-  (*   econstructor. *)
-  (*   eapply (IHa v bs (Ecast a t) i). *)
-  - (* field *)
     inv H.
-    admit. (* inv H4. *)
-    admit.
+    inv H0.
+    eapply eval_Elvalue.
+    eapply eval_Ederef; eauto.
+    simpl in *.
+    destruct H1.
+    eapply deref_loc_value; eauto.
+    eapply deref_loc_reference; eauto.
+    eapply deref_loc_copy; eauto.
+    eapply deref_loc_bitfield; eauto.
+  - inv H.
+    ** econstructor. eapply IHa; eauto.
+       rewrite <-(transf_types_eq a x); eauto.
+    ** inversion H0.
+  - (* field struct *)
+    inv H.
+
+    {
+      inv H0.
+      simpl in *.
+      eapply eval_Elvalue.
+      eapply eval_Efield_struct; eauto.
+      rewrite (transf_types_eq a x) in H5; eauto.
+      assert (SUB: CStan.prog_comp_env prog = ge); eauto; rewrite SUB in *.
+      rewrite comp_env_preserved in *; eauto.
+      assert (SUB: CStan.prog_comp_env prog = ge); eauto; rewrite SUB in *.
+      rewrite comp_env_preserved in *; eauto.
+      destruct H1.
+      eapply deref_loc_value; eauto.
+      eapply deref_loc_reference; eauto.
+      eapply deref_loc_copy; eauto.
+      eapply deref_loc_bitfield; eauto.
+    }
   - (* Eaddrof *)
     inv H.
     inv H0.
   - (* Eunop expressions *)
-    inv H.                               (* invert with CStan.eval_Eunop -- we must additionally show CStan.eval_lvalue is invalid. *)
-    econstructor.                        (* apply Clight.eval_Eunop -- we must additionally show Cop.sem_unary_operation *)
-    apply (IHa v1 bs x EQ H4).       (* Eunop is then shown to be valid by inductive case of it's argument *)
-    rewrite (transf_types_eq a x) in H5; eauto. (* Cop.sem_unary_operation is true by transf_types_eq, so long as EQ *)
-    inv H0.                                     (* CStan.eval_lvalue is invalid. *)
+    inv H.
+    econstructor.
+    apply (IHa v1 bs x TAR MTMP EQ H4).
+    (* Cop.sem_unary_operation is true by transf_types_eq, so long as EQ *)
+    rewrite (transf_types_eq a x) in H5; eauto.
+    inv H0.
 
   - (* Ebinop expressions *)
     inv H.                                 (* invert with CStan.eval_Ebinop *)
-    Focus 2. inv H0.                       (* this also pattern-matches on the invalid CStan.eval_lvalue -- just deal with that now. *)
-    econstructor.                          (* apply Clight.eval_Ebinop *)
-    apply (IHa1 v1 bs x  EQ H5).        (* The first argument is then proven true by the first inductive case*)
-    apply (IHa2 v2 bs x0 EQ1 H6).      (* The second argument is then proven true by the second inductive case*)
-
-    rewrite (transf_types_eq a1 x ) in H7. (* we additionally need to show that Cop.sem_binary_operation is true. *)
+    (* this also pattern-matches on the invalid CStan.eval_lvalue -- just deal with that now. *)
+    2:{ inv H0. }
+    econstructor; eauto.
+    rewrite (transf_types_eq a1 x ) in H7.
     rewrite (transf_types_eq a2 x0) in H7.
     rewrite comp_env_preserved.
     eauto.
@@ -277,19 +336,28 @@ Proof.
     rewrite alignof_equiv.
     constructor.
     inv H0.
-Admitted.
+  - inv H.
+    { inv H0. }
+    econstructor. eauto.
+Qed.
 
 Lemma eval_lvalue_correct:
-  forall e le m a b ofs target ta bf
+  forall e le m a b ofs bf target ta
   (TRE: transf_etarget_expr (prog_target prog) a = OK ta),
-    CStanSemanticsTarget.eval_lvalue ge e le m target a b ofs bf ->
-    CStanSemanticsBackend.eval_lvalue tge e le m ta b ofs bf.
+  CStanSemanticsTarget.eval_lvalue ge e le m target a b ofs bf -> CStanSemanticsBackend.eval_lvalue tge e le m ta b ofs bf.
 Proof.
   intros e le m a.
-  induction a; intros; monadInv TRE; try (inv H).
-  - econstructor. eauto.
-  - eapply CStanSemanticsBackend.eval_Evar_global; eauto.
-    rewrite symbols_preserved; eauto.
+  induction a; intros; try monadInv TRE; try (inv H).
+  - eapply eval_Evar_local; eauto.
+  - eapply eval_Evar_global; eauto.
+    rewrite symbols_preserved; auto.
+  - eapply eval_Ederef.
+    eapply eval_expr_correct; eauto.
+  - eapply eval_Efield_struct.
+    eapply eval_expr_correct; eauto.
+    rewrite (transf_types_eq a x) in *; eauto.
+    rewrite comp_env_preserved in *; eauto.
+    rewrite comp_env_preserved in *; eauto.
 Qed.
 
 Lemma types_correct:
@@ -308,53 +376,54 @@ Proof.
   edestruct (Genv.find_funct_match (proj1 TRANSL)) as (ctx' & tf & A & B & C'); eauto.
 Qed.
 
-(* Lemma match_cont_call_cont: *)
-(*   forall k tk , *)
-(*   match_cont k tk  -> *)
-(*   match_cont (CStanSemanticsTarget.call_cont k) (call_cont tk) . *)
-(* Proof. *)
-(*   induction 1; simpl; auto; intros; econstructor; eauto. *)
-(* Qed. *)
+Lemma match_cont_call_cont:
+  forall bt k tk
+  (MCONT: match_cont bt k tk)
+  (BTOTHER: bt <> BTModel),
+  match_cont bt (call_cont k) (call_cont tk) .
+Proof.
+  induction 1; simpl; auto; intros; econstructor; eauto.
+Qed.
 
-(* Lemma blocks_of_env_preserved: *)
-(*   forall e, CStanSemanticsTarget.blocks_of_env tge e = CStanSemanticsBackend.blocks_of_env ge e. *)
-(* Proof. *)
-(*   intros; unfold blocks_of_env, CStanSemanticsBackend.blocks_of_env. *)
-(*   unfold block_of_binding, CStanSemanticsBackend.block_of_binding. *)
-(*   rewrite comp_env_preserved. auto. *)
-(* Qed. *)
+Lemma blocks_of_env_preserved:
+  forall e, blocks_of_env tge e = blocks_of_env ge e.
+Proof.
+  intros; unfold blocks_of_env, CStanSemanticsBackend.blocks_of_env.
+  unfold block_of_binding, CStanSemanticsBackend.block_of_binding.
+  rewrite comp_env_preserved. auto.
+Qed.
 
-(* Lemma transf_sem_cast_inject: *)
-(*   forall f tf x tx v v' m, *)
-(*   transf_expression x = OK tx -> *)
-(*   transf_function f = OK tf -> *)
-(*   Cop.sem_cast v (CStan.typeof x) (CStan.fn_return f) m = Some v' -> *)
-(*   Cop.sem_cast v (typeof tx) (fn_return tf) m = Some v'. *)
-(* Proof. *)
-(*   intros. *)
-(*   generalize (types_correct _ _ H); intro. *)
-(*   monadInv H0. simpl in *. *)
-(*   rewrite <- H2. *)
-(*   auto. *)
-(* Qed. *)
+Lemma transf_sem_cast_inject:
+  forall f tf x tx v v' m,
+  transf_etarget_expr (prog_target prog) x = OK tx ->
+  transf_function (prog_target prog) f = OK tf ->
+  Cop.sem_cast v (CStan.typeof x) (CStan.fn_return f) m = Some v' ->
+  Cop.sem_cast v (typeof tx) (fn_return tf) m = Some v'.
+Proof.
+  intros.
+  generalize (types_correct _ _ H); intro.
+  monadInv H0. simpl in *.
+  rewrite <- H2.
+  auto.
+Qed.
 
-(* Lemma alloc_variables_preserved: *)
-(*   forall e m params e' m', *)
-(*   CStanSemanticsBackend.alloc_variables ge e m params e' m' -> *)
-(*   alloc_variables tge e m params e' m'. *)
-(* Proof. *)
-(*   induction 1; econstructor; eauto. rewrite comp_env_preserved; auto. *)
-(* Qed. *)
+Lemma alloc_variables_preserved:
+  forall e m params e' m',
+  CStanSemanticsBackend.alloc_variables ge e m params e' m' ->
+  alloc_variables tge e m params e' m'.
+Proof.
+  induction 1; econstructor; eauto. rewrite comp_env_preserved; auto.
+Qed.
 
-(* Lemma bind_parameters_preserved: *)
-(*   forall e m params args m', *)
-(*   CStanSemanticsBackend.bind_parameters ge e m params args m' -> *)
-(*   bind_parameters tge e m params args m'. *)
-(* Proof. *)
-(*   induction 1; econstructor; eauto. inv H0. *)
-(* - eapply assign_loc_value; eauto. *)
-(* - eapply assign_loc_copy; eauto; rewrite <- comp_env_preserved in *; auto. *)
-(* Qed. *)
+Lemma bind_parameters_preserved:
+  forall e m params args m',
+  CStanSemanticsBackend.bind_parameters ge e m params args m' ->
+  bind_parameters tge e m params args m'.
+Proof.
+  induction 1; econstructor; eauto. inv H0.
+- eapply assign_loc_value; eauto.
+- eapply assign_loc_copy; eauto; rewrite <- comp_env_preserved in *; auto.
+Qed.
 
 Lemma eval_exprlist_correct_simple:
   forall env le es tes tys m vs ta
@@ -375,6 +444,18 @@ Proof.
   rewrite <- H; eauto.
 Qed.
 
+(* Lemma seq_both_transf_statement: *)
+(*   forall s0 s1 sfin *)
+(*   (STARGET: transf_starget_statement s0 = OK s1) *)
+(*   (ETARGET: transf_etarget_statement (prog_target prog) s1 = OK sfin) *)
+(*   , transf_statement (prog_target prog) s0 = OK sfin. *)
+(* Proof. *)
+(*   intros. *)
+(*   inv STARGET. *)
+(*   inv ETARGET. *)
+(*   simpl. *)
+(*   inv H0. *)
+(* Admitted. *)
 
 Lemma step_simulation:
   forall S1 t S2, CStanSemanticsTarget.stepf ge S1 t S2 ->
@@ -382,9 +463,9 @@ Lemma step_simulation:
 Proof.
   induction 1.
 
-  - (* assign *)
+  - (* step_assign *)
     simpl; intros; inv MS; simpl in *; try (monadInv TRS; monadInv EQ; monadInv EQ0).
-    + (* assin in Other block *)
+    + (* other *)
       exists (State tf Sskip tk e le m').
       split.
       eapply plus_one.
@@ -401,7 +482,7 @@ Proof.
       eapply assign_loc_copy; try (rewrite comp_env_preserved); eauto.
       eapply match_regular_states; eauto.
 
-    + (* assign in Model Block *)
+    + (* model *)
       exists (State tf Sskip tk e le m').
       split.
       eapply plus_one.
@@ -418,24 +499,25 @@ Proof.
       eapply assign_loc_copy; try (rewrite comp_env_preserved); eauto.
       eapply match_regular_states_model; eauto.
 
-  - (* set *)
+  - (* step_set *)
     simpl; intros; inv MS; simpl in *.
-    + (* in other *)
-      monadInv TRS; monadInv EQ. (* simpl. monadInv EQ0. *)
+    + (* other *)
+      monadInv TRS; monadInv EQ.
+      destruct (id =? (prog_target prog))%positive eqn:TEQ.
+      (* id = target is impossible *) monadInv EQ2.
+      (* otherwise *) inv EQ2. monadInv EQ0.
       econstructor.
       split. eapply plus_one.
-      destruct (id =? (prog_target prog))%positive eqn:TEQ; monadInv EQ2.
-      monadInv EQ0.
       unfold stepf.
       econstructor.
       eapply eval_expr_correct; eauto.
       eapply match_regular_states; eauto.
-    + (* in model *)
-      monadInv TRS.
-      monadInv EQ.
+    + (* other *)
+      monadInv TRS; monadInv EQ.
+      destruct (id =? (prog_target prog))%positive eqn:TEQ.
+      (* id = target is impossible *) monadInv EQ2.
+      (* otherwise *) inv EQ2. monadInv EQ0.
       econstructor.
-      destruct (id =? (prog_target prog))%positive eqn:TEQ; monadInv EQ2.
-      monadInv EQ0.
       split. eapply plus_one.
       unfold stepf.
       econstructor.
@@ -468,211 +550,608 @@ Proof.
       econstructor; eauto. simpl. congruence. rewrite BS_SYNC; auto.
 
   - (* builtin *)
-    simpl; intros; inv MS; simpl in *; monadInv TRS; admit.
-  - (* seq *)
+    simpl; intros; inv MS; simpl in *; try (monadInv TRS; monadInv EQ; monadInv EQ0).
+    admit.
+    admit.
+
+  - (* step_seq *)
+    simpl; intros; inv MS; simpl in *.
+    + (* other *)
+      monadInv TRS.
+      monadInv EQ; monadInv EQ0.
+      econstructor.
+      split.
+      eapply plus_one.
+      unfold stepf.
+      eapply step_seq.
+      eapply match_regular_states; eauto.
+      unfold transf_statement.
+      rewrite EQ1; simpl; eauto.
+      econstructor.
+      unfold transf_statement.
+      rewrite EQ; simpl; eauto.
+      simpl. eauto.
+    + (* model *)
+      monadInv TRS.
+      monadInv EQ; monadInv EQ0.
+      econstructor.
+      split.
+      eapply plus_one.
+      unfold stepf.
+      eapply step_seq.
+      eapply match_regular_states_model; eauto.
+      unfold transf_statement.
+      rewrite EQ1; simpl; eauto.
+      econstructor.
+      unfold transf_statement.
+      rewrite EQ; simpl; eauto.
+      simpl. eauto.
+
+  - (* step_skip_seq *)
+    simpl; intros; inv MS; simpl in *; try (monadInv TRS; monadInv EQ; monadInv EQ0).
+    + (* other *)
+      inv MCONT.
+      econstructor.
+      split.
+      eapply plus_one.
+      unfold stepf.
+      eapply step_skip_seq.
+      eapply match_regular_states; eauto.
+    + (* model *)
+      inv MCONT.
+      econstructor.
+      split.
+      eapply plus_one.
+      unfold stepf.
+      eapply step_skip_seq.
+      eapply match_regular_states_model; eauto.
+
+  - (* step_continue_seq *)
+    simpl; intros; inv MS; simpl in *; try (monadInv TRS; monadInv EQ; monadInv EQ0).
+    + (* other *)
+      inv MCONT.
+      econstructor.
+      split.
+      eapply plus_one.
+      unfold stepf.
+      eapply step_continue_seq.
+      eapply match_regular_states; eauto.
+    + (* model *)
+      inv MCONT.
+      econstructor.
+      split.
+      eapply plus_one.
+      unfold stepf.
+      eapply step_continue_seq.
+      eapply match_regular_states_model; eauto.
+
+  - (* step_break_seq *)
+    simpl; intros; inv MS; simpl in *; try (monadInv TRS; monadInv EQ; monadInv EQ0).
+    + (* other *)
+      inv MCONT.
+      econstructor.
+      split.
+      eapply plus_one; unfold stepf.
+      eapply step_break_seq.
+      eapply match_regular_states; eauto.
+    + (* model *)
+      inv MCONT.
+      econstructor.
+      split.
+      eapply plus_one; unfold stepf.
+      eapply step_break_seq.
+      eapply match_regular_states_model; eauto.
+  - (* step_ifthenelse *)
+    simpl; intros; inv MS; simpl in *; try (monadInv TRS; monadInv EQ; monadInv EQ0).
+    + (* other *)
+      econstructor.
+      split.
+      eapply plus_one; unfold stepf.
+      econstructor.
+      eapply eval_expr_correct; eauto.
+      generalize (types_correct _ _ EQ1); intro.
+      rewrite <- H1; eauto.
+      eapply match_regular_states; eauto.
+      destruct b; eauto.
+      destruct EQ0; eauto.
+      unfold transf_statement.
+      rewrite EQ; simpl; eauto.
+      unfold transf_statement.
+      rewrite EQ2; simpl; eauto.
+    + (* model*)
+      econstructor.
+      split.
+      eapply plus_one; unfold stepf.
+      econstructor.
+      eapply eval_expr_correct; eauto.
+      generalize (types_correct _ _ EQ1); intro.
+      rewrite <- H1; eauto.
+      eapply match_regular_states_model; eauto.
+      destruct b; eauto.
+      destruct EQ0; eauto.
+      unfold transf_statement.
+      rewrite EQ; simpl; eauto.
+      unfold transf_statement.
+      rewrite EQ2; simpl; eauto.
+
+  - (* step_loop *)
+    simpl; intros; inv MS; simpl in *; try (monadInv TRS; monadInv EQ; monadInv EQ0).
+    + (* other *)
+      econstructor.
+      split.
+      eapply plus_one; unfold stepf.
+      eapply step_loop.
+      eapply match_regular_states; eauto.
+      unfold transf_statement.
+      rewrite EQ1; simpl; eauto.
+      simpl.
+      eapply match_Kloop1; eauto.
+      unfold transf_statement.
+      rewrite EQ1; simpl; eauto.
+      unfold transf_statement.
+      rewrite EQ; simpl; eauto.
+    + (* model *)
+      econstructor.
+      split.
+      eapply plus_one; unfold stepf.
+      eapply step_loop.
+      eapply match_regular_states_model; eauto.
+      unfold transf_statement.
+      rewrite EQ1; simpl; eauto.
+      simpl.
+      eapply match_Kloop1; eauto.
+      unfold transf_statement.
+      rewrite EQ1; simpl; eauto.
+      unfold transf_statement.
+      rewrite EQ; simpl; eauto.
+
+  - (* step_skip_or_continue_loop1 *)
+    simpl; intros; inv MS; simpl in *; inv MCONT.
+    + (* other *)
+      monadInv TRS. monadInv H4. monadInv H6.
+      destruct H eqn:F.
+      econstructor; split.
+      eapply plus_one; unfold stepf.
+      eapply step_skip_or_continue_loop1.
+      monadInv TRF; monadInv EQ; monadInv EQ0; eauto.
+      eapply match_regular_states; eauto.
+      unfold transf_statement.
+      rewrite EQ3; simpl; eauto.
+      eapply match_Kloop2; eauto.
+      unfold transf_statement.
+      rewrite EQ1; simpl; eauto.
+      unfold transf_statement.
+      rewrite EQ3; simpl; eauto.
+
+      econstructor; split.
+      eapply plus_one; unfold stepf.
+      eapply step_skip_or_continue_loop1.
+      monadInv TRF; monadInv EQ; monadInv EQ0; eauto.
+      eapply match_regular_states; eauto.
+      unfold transf_statement.
+      rewrite EQ3; simpl; eauto.
+      eapply match_Kloop2; eauto.
+      unfold transf_statement.
+      rewrite EQ1; simpl; eauto.
+      unfold transf_statement.
+      rewrite EQ3; simpl; eauto.
+
+    + (* model *)
+      monadInv TRS. monadInv H4. monadInv H6.
+      destruct H eqn:F.
+      econstructor; split.
+      eapply plus_one; unfold stepf.
+      eapply step_skip_or_continue_loop1.
+      monadInv TRF; monadInv EQ; monadInv EQ0; eauto.
+      eapply match_regular_states_model; eauto.
+      unfold transf_statement.
+      rewrite EQ3; simpl; eauto.
+      eapply match_Kloop2; eauto.
+      unfold transf_statement.
+      rewrite EQ1; simpl; eauto.
+      unfold transf_statement.
+      rewrite EQ3; simpl; eauto.
+
+      econstructor; split.
+      eapply plus_one; unfold stepf.
+      eapply step_skip_or_continue_loop1.
+      monadInv TRF; monadInv EQ; monadInv EQ0; eauto.
+      eapply match_regular_states_model; eauto.
+      unfold transf_statement.
+      rewrite EQ3; simpl; eauto.
+      eapply match_Kloop2; eauto.
+      unfold transf_statement.
+      rewrite EQ1; simpl; eauto.
+      unfold transf_statement.
+      rewrite EQ3; simpl; eauto.
+
+  - (* step_break_loop1 *)
+    simpl; intros; inv MS; simpl in *; monadInv TRS; monadInv EQ; monadInv EQ0; inv MCONT.
+    + (* other *)
+      econstructor. split.
+      eapply plus_one; unfold stepf.
+      eapply step_break_loop1; eauto.
+      eapply match_regular_states; eauto.
+    + (* model *)
+      econstructor. split.
+      eapply plus_one; unfold stepf.
+      eapply step_break_loop1; eauto.
+      eapply match_regular_states_model; eauto.
+
+  - (* step_skip_loop2 *)
+    simpl; intros; inv MS; simpl in *; monadInv TRS; monadInv EQ; monadInv EQ0; inv MCONT.
+    + (* other *)
+      econstructor.
+      split.
+      eapply plus_one; unfold stepf.
+      eapply step_skip_loop2.
+      eapply match_regular_states; eauto.
+      unfold transf_statement.
+      simpl.
+      monadInv H3.
+      monadInv H5.
+      rewrite EQ.
+      rewrite EQ1.
+      simpl.
+      rewrite EQ0.
+      rewrite EQ2.
+      simpl.
+      auto.
+    + (* model *)
+      econstructor.
+      split.
+      eapply plus_one; unfold stepf.
+      eapply step_skip_loop2.
+      eapply match_regular_states_model; eauto.
+      unfold transf_statement.
+      simpl.
+      monadInv H3.
+      monadInv H5.
+      rewrite EQ.
+      rewrite EQ1.
+      simpl.
+      rewrite EQ0.
+      rewrite EQ2.
+      simpl.
+      auto.
+
+  - (* step_break_loop2 *)
+    simpl; intros; inv MS; simpl in *; monadInv TRS; monadInv EQ; monadInv EQ0; inv MCONT.
+    + (* other *)
+      econstructor.
+      split. eapply plus_one; unfold stepf.
+      eapply  step_break_loop2.
+      eapply match_regular_states; eauto.
+    + (* model *)
+      econstructor.
+      split. eapply plus_one; unfold stepf.
+      eapply  step_break_loop2.
+      eapply match_regular_states_model; eauto.
+
+  - (* step_return_0 *)
+    simpl; intros; inv MS; simpl in *; monadInv TRS; monadInv EQ; monadInv EQ0.
+    + (* other *)
+      econstructor.
+      split. eapply plus_one; unfold stepf.
+      eapply step_return_0; eauto. rewrite blocks_of_env_preserved. eauto.
+      eapply match_return_state; eauto.
+      eapply match_cont_call_cont; eauto.
+      simpl. congruence.
+    + (* model *)
+      econstructor.
+      split. eapply plus_one; unfold stepf.
+      eapply step_return_0; eauto. rewrite blocks_of_env_preserved. eauto.
+      eapply match_return_state_model; eauto.
+      eapply match_cont_call_cont; eauto.
+
+  - (* step_return_1 *)
+    (* intros; inv MS. *)
+    simpl; intros; inv MS; simpl in *.
+    + (* other *)
+      monadInv TRS. monadInv EQ. monadInv EQ0. monadInv EQ1.
+      econstructor.
+      split. eapply plus_one; unfold stepf.
+      eapply step_return_1.
+      eapply eval_expr_correct; eauto.
+      eapply transf_sem_cast_inject; eauto.
+      rewrite blocks_of_env_preserved. eauto.
+      eapply match_return_state; eauto.
+      eapply match_cont_call_cont; eauto.
+      simpl; congruence.
+    + (* model *)
+      simpl in *; congruence.
+
+  - (* step_skip_call *)
+    simpl; intros; inv MS; simpl in *; monadInv TRS; monadInv EQ; monadInv EQ0.
+    + (* other *)
+      econstructor.
+      split. eapply plus_one; unfold stepf.
+      econstructor.
+      unfold CStanCont.is_call_cont in H.
+      assert (is_call_cont tk). inv MCONT; simpl in *; auto; try congruence.
+      exact H2.
+      rewrite blocks_of_env_preserved. eauto.
+      eapply match_return_state; eauto.
+    + (* model *)
+      simpl in *; congruence.
+  - (* step_skip_call_model *)
+    simpl; intros; inv MS; simpl in *; monadInv TRS; monadInv EQ; monadInv EQ0.
+    + (* other *)
+      simpl in *; congruence.
+    + (* model *)
+      inv MCONT; simpl in H; destruct H.
+      admit. (* we don't want this state to arrive because we don't want to stop the program during the model block *)
+      congruence.
+      econstructor.
+      split.
+      * eapply plus_left'; unfold stepf.
+        econstructor.
+        eapply plus_one; unfold stepf.
+        econstructor.
+        eapply eval_Etempvar; eauto.
+        simpl in *.
+        admit. (*I think I need to strengthen this argument*)
+        rewrite blocks_of_env_preserved; eauto.
+        simpl; congruence.
+      * (* eapply match_regular_states_model. *) (* need to pop off this continuation before getting to the match_return_state_model but not sure how *)
+        eapply match_return_state_model.
+        admit. (* now, I think because I didn't pop off the kcall, we have a funny state here that doesn't make sense *)
+        simpl in *.
+        eapply match_Kcall; auto.
+        congruence.
+  - (* step_skip_break_switch *)
+    simpl; intros; inv MS; simpl in *; monadInv TRS.
+    + (* other *)
+       destruct H as [Hskip | Hbreak] eqn:Hboth.
+       * (* skip *)
+         rewrite Hskip in EQ.
+         inversion EQ. rewrite <- H1 in EQ0.
+         inversion EQ0.
+         inversion MCONT.
+         exists (State tf Sskip tk0 e le m).
+         split.
+         eapply plus_one. unfold stepf.
+         eapply step_skip_break_switch.
+         auto.
+         eapply match_regular_states; simpl in *; eauto.
+
+       * (* break -- how to fold this into a repeat? *)
+         rewrite Hbreak in EQ.
+         inversion EQ. rewrite <- H1 in EQ0.
+         inversion EQ0.
+         inversion MCONT.
+         exists (State tf Sskip tk0 e le m).
+         split.
+         eapply plus_one. unfold stepf.
+         eapply step_skip_break_switch.
+         auto.
+         eapply match_regular_states; simpl in *; eauto.
+    + (* model *)
+       destruct H as [Hskip | Hbreak] eqn:Hboth.
+       * (* skip *)
+         rewrite Hskip in EQ.
+         inversion EQ. rewrite <- H1 in EQ0.
+         inversion EQ0.
+         inversion MCONT.
+         exists (State tf Sskip tk0 e le m).
+         split.
+         eapply plus_one. unfold stepf.
+         eapply step_skip_break_switch.
+         auto.
+         eapply match_regular_states_model; simpl in *; eauto.
+
+       * (* break -- how to fold this into a repeat? *)
+         rewrite Hbreak in EQ.
+         inversion EQ. rewrite <- H1 in EQ0.
+         inversion EQ0.
+         inversion MCONT.
+         exists (State tf Sskip tk0 e le m).
+         split.
+         eapply plus_one. unfold stepf.
+         eapply step_skip_break_switch.
+         auto.
+         eapply match_regular_states_model; simpl in *; eauto.
+  - (* step_continue_switch *)
+    intros; simpl; intros; inv MS; simpl in *; monadInv TRS; monadInv EQ; monadInv EQ0.
+    + (* other *)
+      inv MCONT.
+      exists (State tf Scontinue tk0 e le m).
+      split. eapply plus_one; unfold stepf.
+      econstructor.
+      eapply match_regular_states; eauto.
+    + (* model *)
+      inv MCONT.
+      exists (State tf Scontinue tk0 e le m).
+      split. eapply plus_one; unfold stepf.
+      econstructor.
+      eapply match_regular_states_model; eauto.
+
+  - (* step_internal_function *)
+    (* other-only *)
+    intros; simpl; intros; inv MS; simpl in *.
+    monadInv TRFD.
+    exists (State x (fn_body x) tk e (create_undef_temps (fn_temps x)) m1).
+    (* econstructor. *)
+    split. eapply plus_one; unfold stepf.
+    eapply step_internal_function.
+    inversion H.
+    assert (tr_function f x).
+      intros; monadInv EQ.
+      econstructor; eauto.
+    inv H4.
+    econstructor; try (rewrite H7); try (rewrite H8); monadInv EQ; eauto.
+    eapply alloc_variables_preserved; eauto.
+    eapply bind_parameters_preserved; eauto.
+    assert (create_undef_temps (fn_temps x) = le). {
+      (* lost information about (le = create_undef_temps (fn_temps x)) *)
+      Search create_undef_temps.
+      admit.
+    }.
+    admit.
+    (* rewrite H1. *)
+    (* induction (get_blockstate ta). *)
+    (* apply get_blockstate in ta. *)
+    (* eapply match_regular_states; eauto. *)
+    (* admit. (* transf_statement *) *)
+
+    (* admit. (* transf_statement *) *)
+    (* (* Search create_undef_temps. *) *)
+    (* (* eapply match_regular_states; eauto. *) *)
+    (* admit. *)
+
+  - (* step_internal_function_model *)
+    (* model-only *)
+    intros; simpl; intros; inv MS; simpl in *.
+    monadInv TRFD.
+    econstructor.
+    split. eapply plus_one; unfold stepf.
+    eapply step_internal_function.
+    inversion H.
+    assert (tr_function f x).
+      intros; monadInv EQ.
+      econstructor; eauto.
+    inv H4.
+    econstructor; try (rewrite H7); try (rewrite H8); monadInv EQ; eauto.
+    eapply alloc_variables_preserved; eauto.
+    eapply bind_parameters_preserved; eauto.
+    (* lost information about (le = create_undef_temps (fn_temps x)) *)
+    (* Search create_undef_temps. *)
+    (* eapply match_regular_states_model; eauto. *)
+    admit.
+
+  - (* step_external_function *)
+    intros.
+    destruct ta.
+    * (* model *)
+      inv MS.
+      monadInv TRFD.
+      exists (Returnstate vres tk m').
+      split. eapply plus_one. eapply step_external_function. eapply Events.external_call_symbols_preserved; eauto. apply senv_preserved.
+      unfold transf_external in EQ.
+      induction ef; monadInv EQ; eauto.
+      eapply match_return_state_model; eauto.
+      simpl.
+      auto.
+      admit. (* needed to do inversion, maybe on MCONT, much earlier to propagate the block_state *)
+    * (* model *)
+      inv MS.
+      monadInv TRFD.
+      exists (Returnstate vres tk m').
+      split. eapply plus_one. eapply step_external_function. eapply Events.external_call_symbols_preserved; eauto. apply senv_preserved.
+      unfold transf_external in EQ.
+      induction ef; monadInv EQ; eauto.
+      eapply match_return_state; eauto.
+
+  - (* step_returnstate *)
+    intros. inv MS.
+    + (* other *)
+      inv MCONT.
+      * econstructor. split. apply plus_one. eapply step_returnstate.
+        eapply match_regular_states; eauto. (* lost the fn_blocktype too early *)
+        admit.
+        monadInv H6.
+        inversion H8.
+        ** (* Kstop *) econstructor.
+        ** (* Kseq *) econstructor; eauto.
+           (* we don't have a link from match_cont (fn_blocktype f) to (get_blockstate Other)*)
+           (* what we need is to loosen get_blockstate to be an inductive type that introduces that bt <> BTModel, I think *)
+           admit.
+        ** (* Kloop1 *) econstructor; eauto. admit.
+        ** (* Kloop2 *) econstructor; eauto. admit.
+        ** (* Kswitch *) econstructor; eauto. admit.
+        ** (* Kcall *) econstructor; eauto.
+        ** (* Kcall to Kseq *) econstructor; eauto. (* here, I think the above solution would fix this as well *) admit.
+      * discriminate.
+    + (* model *)
+      simpl in *.
+      inv MCONT.
+      * simpl in H7. congruence.
+      * simpl in *.
+        econstructor. split.
+        (* we are in the returnstate of the model. Kcall will continue in the outer function. *)
+        (* We want to step through the known continuation of the model's Kseq to get to the  *)
+        (* final return of the prog_target prog but we get an error of not finding the correct *)
+        eapply plus_left'. unfold stepf.
+        admit. (* We need a way to have something like a step_return_1_model otherwise we can't unify *)
+                (* stepping through the continuation here, I think. *)
+        eapply plus_one. unfold stepf.
+        eapply step_returnstate.
+        admit. (* everything gets messy here. eapply step_returnstate makes sense, but *)
+               (* gives me this ridiculous statement E0 = Eapp _ E0 ... I need to review eventing *)
+        eapply match_regular_states_model; eauto.
+        admit. (* lost the blocktype f = BTModel *)
+        (* Search set_opttemp. *)
+        admit. (* hmm... I guess the continuation doesn't add any additional context *)
+               (* about setting the ident in this goal.... *)
+        simpl in *.
+        admit. (* and, again, lost that blocktype f = BTModel *)
+
+        (* (* now deal with the epilouge *) *)
+        (* * inv MCONT; simpl in *. *)
+        (* ** admit. *)
+        (* ** eapply match_regular_states_model; eauto. *)
+        (* *** rewrite H6. *)
+        (*   admit. (* transf_function (prog_target prog) f = OK ? *) *)
+        (* *** admit. (* transf_statement (prog_target prog) Sskip = OK ? *) *)
+        (* *** admit. (* fn_blocktype f = BTModel *) *)
+        (* *** admit. (* (set_opttemp optid v le) ! (prog_target prog) = Some (Vfloat ta0) *) *)
+        (* *** admit. (* (set_opttemp optid v le) ! (prog_target prog) = Some (Vfloat ta0) *) *)
+  - (* step_target *)
+    intros; inv MS; monadInv TRS; monadInv EQ; monadInv EQ0; simpl in *.
+    + (* other *) discriminate.
+    + (* model *)
+      econstructor. split. eapply plus_left'. unfold stepf.
+      eapply step_set.
+      eapply eval_expr_correct.
+      simpl in *.
+      (* need to review the workshop sequences module... *)
 
 
 
 
-  (*   eapply eval_expr_correct; eauto. *)
-  (*   exploit eval_expr_correct; eauto; intro. *)
-  (*   exploit eval_exprlist_correct_simple; eauto. intro tvargs. *)
-  (*   exploit functions_translated; eauto. intros [tfd [P Q]]. *)
-  (*   econstructor. split. eapply plus_one. eapply step_call with (fd := tfd). *)
-  (*   generalize (types_correct _ _ EQ); intro TYA. rewrite<-TYA. eauto. *)
-  (*   eauto. eauto. eauto. *)
-  (*   rewrite (type_of_fundef_preserved fd); eauto. *)
-  (*   eapply match_call_state; eauto. *)
-  (*   econstructor; eauto. *)
+      econstructor. split. eapply plus_one. unfold stepf.
+      eapply step_set.
+      eapply eval_expr_correct.
+      admit. (*not sure how to do this one*)
+      admit.
 
-  (* - (* builtin *) *)
-  (*   intros; inv MS. *)
-  (*   monadInv TRS. *)
-  (*   exists (State tf Sskip tk e (set_opttemp optid vres le) m'). *)
-  (*   split. eapply plus_one. unfold step1. *)
-  (*   eapply step_builtin. *)
-  (*   eapply eval_exprlist_correct_simple; eauto. *)
-  (*   eapply Events.external_call_symbols_preserved; eauto. apply senv_preserved. *)
-  (*   eapply match_regular_states; eauto. *)
-  (* - (* sequence seq *) *)
-  (*   intros. *)
-  (*   inv MS; monadInv TRS. *)
-  (*   exists (State tf x (Kseq x0 tk) e le m). *)
-  (*   split. *)
-  (*   eapply plus_one. *)
-  (*   unfold step1. *)
-  (*   eapply step_seq. *)
-  (*   eapply match_regular_states; eauto. *)
-  (*   econstructor; eauto. *)
-  (* - (* skip sequence *) *)
-  (*   intros. *)
-  (*   inv MS; monadInv TRS. *)
-  (*   inv MCONT. *)
-  (*   exists (State tf ts tk0 e le m). *)
-  (*   split. *)
-  (*   eapply plus_one. *)
-  (*   unfold step1. *)
-  (*   eapply step_skip_seq. *)
-  (*   eapply match_regular_states; eauto. *)
-  (* - (* continue sequence *) *)
-  (*   intros; inv MS; monadInv TRS. *)
-  (*   inv MCONT. *)
-  (*   exists (State tf Scontinue tk0 e le m). *)
-  (*   split. *)
-  (*   eapply plus_one. *)
-  (*   unfold step1. *)
-  (*   eapply step_continue_seq. *)
-  (*   eapply match_regular_states; eauto. *)
-  (* - (* break sequence *) *)
-  (*   intros; inv MS; monadInv TRS. *)
-  (*   inv MCONT. *)
-  (*   exists (State tf Sbreak tk0 e le m). *)
-  (*   split. *)
-  (*   eapply plus_one; unfold step1. *)
-  (*   eapply step_break_seq. *)
-  (*   eapply match_regular_states; eauto. *)
-  (* - (* if then else *) *)
-  (*   intros; inv MS; monadInv TRS. *)
-  (*   econstructor. *)
-  (*   split. *)
-  (*   eapply plus_one; unfold step1. *)
-  (*   econstructor. *)
-  (*   eapply eval_expr_correct; eauto. *)
-  (*   generalize (types_correct _ _ EQ); intro. *)
-  (*   rewrite <- H1; eauto. *)
-  (*   eapply match_regular_states; eauto. *)
-  (*   destruct b; eauto. *)
-  (* - (* step_loop *) *)
-  (*   intros; inv MS; monadInv TRS. *)
-  (*   exists (State tf x (Kloop1 x x0 tk) e le m). *)
-  (*   split. *)
-  (*   eapply plus_one; unfold step1. *)
-  (*   eapply step_loop. *)
-  (*   eapply match_regular_states; eauto. *)
-  (*   eapply match_Kloop1; eauto. *)
-  (* - (* step_skip_or_continue_loop1 *) *)
-  (*   intros. inv MS; inv MCONT; destruct H; *)
-  (*   repeat ( *)
-  (*     econstructor; split; *)
-  (*     try (eapply plus_one; unfold step1; *)
-  (*       eapply step_skip_or_continue_loop1; *)
-  (*       monadInv TRF; monadInv TRS; eauto); *)
-  (*     eapply match_regular_states; eauto; eapply match_Kloop2; eauto *)
-  (*   ). *)
 
-  (* - (* step_break_loop1 *) *)
-  (*   intros; inv MS; monadInv TRS; inv MCONT. *)
-  (*   econstructor. split. *)
-  (*   eapply plus_one; unfold step1. *)
-  (*   eapply step_break_loop1; eauto. *)
-  (*   eapply match_regular_states; eauto. *)
-  (* - (* step_skip_loop2 *) *)
-  (*   intros; inv MS; monadInv TRS; inv MCONT. *)
-  (*   exists (State tf (Sloop ts1 ts2) tk0 e le m). *)
-  (*   split. *)
-  (*   eapply plus_one; unfold step1. *)
-  (*   eapply step_skip_loop2. *)
-  (*   eapply match_regular_states; eauto. *)
-  (*   simpl. rewrite H2. rewrite H4. auto. *)
 
-  (* - (* step_break_loop2 *) *)
-  (*   intros; inv MS; monadInv TRS; inv MCONT. *)
-  (*   exists (State tf Sskip tk0 e le m). *)
-  (*   split. eapply plus_one; unfold step1. *)
-  (*   eapply  step_break_loop2. *)
-  (*   eapply match_regular_states; eauto. *)
 
-  (* - (* step_return_0 *) *)
-  (*   intros; inv MS; monadInv TRS. *)
-  (*   exists (Returnstate Values.Vundef (call_cont tk) m'). *)
-  (*   split. eapply plus_one; unfold step1. *)
-  (*   eapply step_return_0; eauto. rewrite blocks_of_env_preserved. eauto. *)
-  (*   eapply match_return_state; eauto. *)
-  (*   eapply match_cont_call_cont; eauto. *)
-  (* - (* step_return_1 *) *)
-  (*   intros; inv MS. *)
-  (*   exists (Returnstate v' (call_cont tk) m'). *)
-  (*   monadInv TRS. *)
-  (*   split. eapply plus_one; unfold step1. *)
-  (*   econstructor; eauto. *)
-  (*   eapply eval_expr_correct; eauto. *)
-  (*   eapply transf_sem_cast_inject; eauto. *)
-  (*   rewrite blocks_of_env_preserved. eauto. *)
-  (*   eapply match_return_state; eauto. *)
-  (*   eapply match_cont_call_cont; eauto. *)
 
-  (* - (* step_skip_call *) *)
-  (*   intros; inv MS; monadInv TRS. *)
-  (*   econstructor. *)
-  (*   split. eapply plus_one; unfold step1. *)
-  (*   econstructor. *)
-  (*   unfold CStanSemanticsTarget.is_call_cont in H. *)
-  (*   assert (is_call_cont tk). inv MCONT; simpl in *; auto. auto. *)
-  (*   rewrite blocks_of_env_preserved. eauto. *)
-  (*   eapply match_return_state; eauto. *)
+      inv H.
+      (* step the expression *)
+      monadInv EQ.
+        eapply step_assign; eauto.
+        eapply eval_lvalue_correct; eauto.
+        (* assert (eval_lvalue tge e le (Evar (prog_target prog) tdouble )). *)
+      (*   eapply eval_expr_correct; eauto. *)
+      (* inv H2. *)
+      (* eapply assign_loc_value; eauto. *)
+      (* eapply assign_loc_copy; try (rewrite comp_env_preserved); eauto. *)
+      (* eapply match_regular_states; eauto. *)
 
-  (* - (* step_skip_break_switch *) *)
-  (*   intros; inv MS. inv MCONT. *)
-  (*   econstructor. *)
-  (*   split. eapply plus_one; unfold step1. *)
-  (*   econstructor. *)
-  (*   destruct H; simpl in *. *)
-  (*   monadInv TRF; monadInv TRS; eauto. *)
-  (*   monadInv TRF; monadInv TRS; eauto. *)
-  (*   eapply match_regular_states; eauto. *)
 
-  (* - (* step_continue_switch *) *)
-  (*   intros; inv MS; monadInv TRS; inv MCONT. *)
-  (*   exists (State tf Scontinue tk0 e le m). *)
-  (*   split. eapply plus_one; unfold step1. *)
-  (*   econstructor. *)
-  (*   eapply match_regular_states; eauto. *)
+      * (* match the states *)
 
-  (* - (* step_internal_function *) *)
-  (*   intros; inv MS. *)
-  (*   monadInv TRFD. *)
-  (*   exists (State x x.(fn_body) tk e le m1). *)
-  (*   split. eapply plus_one; unfold step1. *)
-  (*   eapply step_internal_function. *)
-  (*   inversion H. *)
-  (*   assert (tr_function f x). { *)
-  (*     intros; monadInv EQ. *)
-  (*     econstructor; eauto. *)
-  (*   }. *)
-  (*   inv H4. *)
-  (*   econstructor; try (rewrite H7); try (rewrite H8); eauto. *)
-  (*   eapply alloc_variables_preserved; eauto. *)
-  (*   eapply bind_parameters_preserved; eauto. *)
-  (*   monadInv EQ; eauto. *)
-  (*   eapply match_regular_states; eauto. *)
-  (*   monadInv EQ. eauto. *)
+Lemma eval_lvalue_correct:
+  forall e le m a b ofs target ta
+  (TRE: transf_etarget_expr (prog_target prog) a = OK ta),
+  CStanSemanticsTarget.eval_lvalue ge e le m target a b ofs -> CStanSemanticsBackend.eval_lvalue tge e le m ta b ofs.
+Proof.
+  intros e le m a.
+  induction a; intros; monadInv TRE; try (inv H).
+  - econstructor. eauto.
+  - eapply CStanSemanticsBackend.eval_Evar_global; eauto.
+    rewrite symbols_preserved; eauto.
+Qed.
 
-  (* - (* step_external_function *) *)
-  (*   intros. inv MS. *)
-  (*   monadInv TRFD. *)
-  (*   exists (Returnstate vres tk m'). *)
-  (*   split. eapply plus_one. eapply step_external_function. eapply Events.external_call_symbols_preserved; eauto. apply senv_preserved. *)
-  (*   eapply match_return_state; eauto. *)
-  (* - (* step_returnstate *) *)
-  (*   intros. inv MS. *)
-  (*   inv MCONT. *)
-  (*   exists (State tfn Sskip tk0 e (set_opttemp optid v le) m). *)
-  (*   split. apply plus_one. eapply step_returnstate. *)
-  (*   eapply match_regular_states; eauto. *)
-  (*   (***************************************************************************************************) *)
-  (* - (* target *) *)
-  (*   intros. inv MS. *)
-  (*   exists (State f (Starget ta) k e le m (CStanSemanticsTarget.Model (Floats.Float.add ta ta'))). *)
-  (*   econstructor. *)
-  (*   split. *)
-  (*   eapply plus_one. *)
-  (*   unfold step1. *)
-  (*   inversion TRS. *)
-  (*   eapply match_regular_states; eauto. *)
-  (*   admit. *)
+
+
+
+
 Admitted.
 
-(*
 Lemma function_ptr_translated:
 (*   forall m0 *)
 (*     (b: block) (f: CStan.fundef) *)
@@ -689,11 +1168,10 @@ Lemma function_ptr_translated:
 (* Admitted. *)
 (*   (* edestruct (Genv.find_funct_ptr_match (proj1 TRANSL)) as (ctx' & tf & A & B & C'); eauto. *) *)
 (* (* Qed. *) *)
-*)
 
 Lemma initial_states_simulation:
   forall S, CStanSemanticsTarget.initial_state prog S ->
-  exists R, CStanSemanticsBackend.initial_state tprog R /\ match_states S R.
+  exists R, CStanSemanticsBackend.initial_state tprog R /\ match_states prog.(prog_target) S R.
 Proof.
   intros. inv H.
   (* exploit function_ptr_translated; eauto. *)
@@ -716,8 +1194,8 @@ Admitted.
 (* Qed. *)
 
 Lemma final_states_simulation:
-  forall S R r,
-  match_states S R -> CStanSemanticsTarget.final_state S r -> final_state R r.
+  forall S R r i,
+  match_states i S R -> CStanSemanticsTarget.final_state S r -> final_state R r.
 Proof.
   intros. inv H0. inv H; inv MCONT; constructor.
 Qed.
